Proved a simple lemma about Valid.

src/AsyncFinish/Typesystem.v
@@ -3,7 +3,17 @@ Require Import Coq.Lists.SetoidList.
 Require Import HJ.Vars.
 Require Import HJ.AsyncFinish.Lang.
 
-Definition IsMap := (NoDupA (Map_TID.eq_key (elt:=task))).
+Inductive IsMap : finish -> Prop :=
+  is_map_def:
+    forall l,
+    NoDupA (Map_TID.eq_key (elt:=task)) l ->
+    IsMap (Node l).
+
+Lemma is_map_nil:
+  IsMap (Node nil).
+Proof.
+  auto using NoDupA_nil, is_map_def.
+Qed.
 
 Inductive Valid: finish -> Prop :=
   | valid_nil:
@@ -19,3 +29,58 @@ Inductive Valid: finish -> Prop :=
     Valid (Node l) ->
     ~ In t (Node l) ->
     Valid (Node ((t,Blocked f)::l)).
+
+Require Import HJ.AsyncFinish.LangExtra.
+
+Lemma in_to_ina:
+  forall t a l, 
+  ~ In t (Node l) ->
+  ~ InA (Map_TID.eq_key (elt:=task)) (t, a) l.
+Proof.
+  intros.
+  apply notin_spec in H.
+  induction l.
+  - intuition.
+    inversion H0.
+  - apply notin_inv in H.
+    destruct a0 as (t', a').
+    destruct H as  (?, (?, ?)).
+    simpl in H0, H.
+    unfold not.
+    intros.
+    inversion H2.
+    + subst.
+      apply Map_TID_Extra.eq_key_unfold in H4; auto.
+    + subst.
+      intuition.
+Qed.
+
+Lemma valid_impl_is_map:
+  forall f,
+  Valid f ->
+  IsMap f.
+Proof.
+  intros f.
+  induction f using finish_ind_strong.
+  - intros.
+    auto using is_map_nil.
+  - intros.
+    inversion H.
+    subst.
+    apply is_map_def.
+    apply NoDupA_cons.
+    + auto using in_to_ina.
+    + apply IHf in H2.
+      inversion H2.
+      assumption.
+  - intros.
+    inversion H.
+    subst.
+    apply is_map_def.
+    apply NoDupA_cons.
+    + auto using in_to_ina.
+    + apply IHf0 in H4.
+      inversion H4.
+      assumption.
+Qed.
+    
